full_context_dependency strikes again

examples/metatheory/norm.fst
@@ -4,14 +4,20 @@ module Norm
 open Prims
 open Stlc
 
-(* need to define the reflexive-transitive closure of step, somehow *)
+(* XXX both multi and red require the --full_context_dependency flag XXX 
+   Compile this file with:
+   ../../bin/fstar.exe --fstar_home ../.. stlc.fst norm.fst --full_context_dependency
+*)
+
+(* Reflexive-transitive closure of step *)
 
 kind Relation (a:Type) = a -> a -> Type
 
-(* CH: for failed attempts to define this see below *)
-assume type multi (a:Type) (r:Relation a) : Relation a
-
-assume val multi_refl : #a:Type -> x:a -> r:Relation a -> Lemma (multi a r x x)
+(* CH: needed to unfold the definition of Relation to make this work;
+   for failed attempts to define this see below *)
+type multi (a:Type) (r:(a -> a -> Type)) : a -> a -> Type =
+  | Multi_refl : x:a -> multi a r x x
+  | Multi_step : x:a -> y:a -> z:a -> r x y -> multi a r y z -> multi a r x z
 
 (*
 Kinds "(_:a -> _:a -> Type)" and "Type" are incompatible
@@ -28,24 +34,7 @@ type multi : 'a:Type -> ('a -> 'a -> Type) -> 'a -> 'a -> Type =
   | Multi_step : x:'a -> y:'a -> z:'a -> r:('a -> 'a -> Type) -> r x y -> multi r y z -> multi r x z
 *)
 
-(*
-norm.fst(10,4-10,14) : Error
-Expected expression of type "(multi #(U811 a r) #(U812 a r _2 _3 _954) #('e813 a r) #('e814 a r))";
-got expression "_954" of type "(multi #a #r #_2 #_3)"
-
-type multi (a:Type) (r:(a -> a -> Type)) : a -> a -> Type =
-  | Multi_refl : x:a -> multi a r x x
-  | Multi_step : x:a -> y:a -> z:a -> r x y -> multi a r y z -> multi a r x z
-*)
-
-(* The Coq definition for multi
-Inductive multi {X:Type} (R: relation X) : relation X :=
-  | multi_refl  : forall (x : X), multi R x x
-  | multi_step : forall (x y z : X),
-                    R x y ->
-                    multi R y z ->
-                    multi R x z.
-*)
+assume val multi_refl : #a:Type -> x:a -> r:Relation a -> Lemma (multi a r x x)
 
 type step_rel (e:exp) (e':exp) : Type = step e == Some e'
 
@@ -59,81 +48,26 @@ val value_halts : v:exp ->
 let value_halts v =
   multi_refl v step_rel
 
-(*
-Expected expression of type "(red #('e818 a r) #('e819 a r))";
-got expression "_964" of type "(red #_0 #_1)"
-*)
-type red : ty -> exp -> Type =
-  | R_bool : e:exp -> red TBool e
-  | R_boolp : e:exp -> red TBool e
-(*
-  | R_arrow : t1:ty -> t2:ty
-               -> e:exp (* {typing empty e = Some (TArrow t1 t2) /\ halts e} *)
-(*               -> (e':exp -> R t1 e' -> Tot (R t2 (EApp e e'))) *)
-               -> red (TArrow t1 t2) e
-*)
-
 (* This has a negative occurrence of R that makes Coq succumb,
    although this definition is just fine (the type decreases);
-   F* should have similar problems at this point
-type R : ty -> exp -> Type =
-  | R_bool : e:exp{typing empty e = Some TBool /\ halts e} -> R TBool e
+   F* should have similar problems as soon as we start checking
+   for negative occurrences. *)
+type red : ty -> exp -> Type =
+  | R_bool : e:exp{typing empty e = Some TBool /\ halts e} -> red TBool e
   | R_arrow : t1:ty -> t2:ty
                -> e:exp{typing empty e = Some (TArrow t1 t2) /\ halts e}
-               -> (e':exp -> R t1 e' -> Tot (R t2 (EApp e e')))
-               -> R (TArrow t1 t2) e
-*)
-(* I agree we should get a negative occurrence error for the above;
-   but the 10(!) errors we get are incomprehensible:
-time ../../bin/fstar.exe --fstar_home ../.. stlc.fst norm.fst --print_implicits
-Error norm.fst(20,13-20,14): The following problems were found:
-	Subtyping check failed; expected type (R #'e819 #'e820); got type (R #_0 #_1) (norm.fst(20,4-20,10))
-Error norm.fst(20,13-20,14): Unconstrained unification variables 'e820,'e819 in type signature (#_0:ty -> #_1:exp -> projectee:_958:(R #_0 #_1){(is_R_bool #'e819 #'e820 _958)} -> Tot e:exp{(((typing empty e) = (Some #ty TBool)) /\ (halts e))}); please add an annotation
-Error norm.fst(21,14-21,16): The following problems were found:
-	Subtyping check failed; expected type (R #'e823 #'e824); got type (R #_0 #_1) (norm.fst(21,4-21,11))
-Error norm.fst(21,14-21,16): Unconstrained unification variables 'e824,'e823 in type signature (#_0:ty -> #_1:exp -> projectee:_960:(R #_0 #_1){(is_R_arrow #'e823 #'e824 _960)} -> Tot ty); please add an annotation
-Error norm.fst(21,23-21,25): The following problems were found:
-	Subtyping check failed; expected type (R #'e825 #'e826); got type (R #_0 #_1) (norm.fst(21,4-21,11))
-Error norm.fst(21,23-21,25): Unconstrained unification variables 'e826,'e825 in type signature (#_0:ty -> #_1:exp -> projectee:_960:(R #_0 #_1){(is_R_arrow #'e825 #'e826 _960)} -> Tot ty); please add an annotation
-Error norm.fst(22,18-22,19): The following problems were found:
-	Subtyping check failed; expected type (R #'e827 #'e828); got type (R #_0 #_1) (norm.fst(21,4-21,11))
-Error norm.fst(22,18-22,19): Unconstrained unification variables 'e834,'e833,'e832,'e831,'e828,'e827 in type signature (#_0:ty -> #_1:exp -> projectee:_960:(R #_0 #_1){(is_R_arrow #'e827 #'e828 _960)} -> Tot e:exp{(((typing empty e) = (Some #ty (TArrow (t1 #'e831 #'e832 projectee) (t2 #'e833 #'e834 projectee)))) /\ (halts e))}); please add an annotation
-Error norm.fst(22,18-22,19): The following problems were found:
-	Subtyping check failed; expected type _960:(R #'e841 #'e842){(is_R_arrow #'e827 #'e828 _960)}; got type _960:(R #_0 #_1){(is_R_arrow #'e835 #'e836 _960)} (norm.fst(21,4-21,11))
-Error unknown(0,0-0,0): Unconstrained unification variables 'e842,'e841,'e840,'e839,'e838,'e837,'e836,'e835 in type signature (#_0:ty -> #_1:exp -> projectee:_960:(R #_0 #_1){(is_R_arrow #'e835 #'e836 _960)} -> Tot (e':exp -> _:(R (t1 #'e837 #'e838 projectee) e') -> Tot (R (t2 #'e839 #'e840 projectee) (EApp (e #'e841 #'e842 projectee) e')))); please add an annotation
-Verified module: Prims
-Verified module: Stlc
-Verified module: Norm
-Error: 10 errors were reported (see above)
-*)
+               -> (e':exp -> red t1 e' -> Tot (red t2 (EApp e e')))
+               -> red (TArrow t1 t2) e
 
-(* My original attempt
-  | R_arrow : e:exp -> t1:ty -> t2:ty{typing empty e = Some (TArrow t1 t2)
-      /\ halts e /\ (forall (e':exp). R t1 e' ==> R t2 (EApp e e'))} ->
-      R (TArrow t1 t2) e
+(* My original attempt -- red' called recursively only in refinement *)
+type red' : ty -> exp -> Type =
+  | R_bool' : e:exp{typing empty e = Some TBool /\ halts e} -> red' TBool e
+  | R_arrow' : e:exp -> t1:ty -> t2:ty{typing empty e = Some (TArrow t1 t2)
+      /\ halts e /\ (forall (e':exp). red' t1 e' ==> red' t2 (EApp e e'))} ->
+      red' (TArrow t1 t2) e
 
-time ../../bin/fstar.exe --fstar_home ../.. stlc.fst norm.fst --print_implicits
-Error norm.fst(20,13-20,14): The following problems were found:
-	Subtyping check failed; expected type (R #'e820 #'e821); got type (R #_0 #_1) (norm.fst(20,4-20,10))
-Error norm.fst(20,13-20,14): Unconstrained unification variables 'e821,'e820 in type signature (#_0:ty -> #_1:exp -> projectee:_958:(R #_0 #_1){(is_R_bool #'e820 #'e821 _958)} -> Tot e:exp{(((typing empty e) = (Some #ty TBool)) /\ (halts e))}); please add an annotation
-Error norm.fst(22,14-22,15): The following problems were found:
-	Subtyping check failed; expected type (R #'e824 #'e825); got type (R #_0 #_1) (norm.fst(22,4-22,11))
-Error norm.fst(22,14-22,15): Unconstrained unification variables 'e825,'e824 in type signature (#_0:ty -> #_1:exp -> projectee:_960:(R #_0 #_1){(is_R_arrow #'e824 #'e825 _960)} -> Tot exp); please add an annotation
-Error norm.fst(22,23-22,25): The following problems were found:
-	Subtyping check failed; expected type (R #'e826 #'e827); got type (R #_0 #_1) (norm.fst(22,4-22,11))
-Error norm.fst(22,23-22,25): Unconstrained unification variables 'e827,'e826 in type signature (#_0:ty -> #_1:exp -> projectee:_960:(R #_0 #_1){(is_R_arrow #'e826 #'e827 _960)} -> Tot ty); please add an annotation
-Error norm.fst(22,32-22,34): The following problems were found:
-	Subtyping check failed; expected type (R #'e828 #'e829); got type (R #_0 #_1) (norm.fst(22,4-22,11))
-Error norm.fst(22,32-22,34): Unconstrained unification variables 'e842,'e841,'e840,'e839,'e837,'e836,'e835,'e834,'e832,'e831,'e829,'e828 in type signature (#_0:ty -> #_1:exp -> projectee:_960:(R #_0 #_1){(is_R_arrow #'e828 #'e829 _960)} -> Tot t2:ty{((((typing empty (e #'e831 #'e832 projectee)) = (Some #ty (TArrow (t1 #'e834 #'e835 projectee) t2))) /\ (halts (e #'e836 #'e837 projectee))) /\ (forall (e':exp). ((R (t1 #'e839 #'e840 projectee) e') ==> (R t2 (EApp (e #'e841 #'e842 projectee) e')))))}); please add an annotation
-Verified module: Prims
-Verified module: Stlc
-Verified module: Norm
-Error: 8 errors were reported (see above)
-../../bin/fstar.exe --fstar_home ../.. stlc.fst norm.fst --print_implicits  2.49s user 0.10s system 17% cpu 14.620 total
-*)
-
-(* In Coq we define R by recursion on the type,
-   we don't have fixpoints in Type in F* though, do we?
+(* In Coq we define R/red by recursion on the type,
+   we don't have fixpoints in Type in F* though (see mailing list discussion)
 The type of R is
 val R : ty -> exp -> Type
 *)
